\documentclass{article}

\usepackage{amsmath}

\title{Week 2 Assignment}
\author{Jiaqi Wang}

\begin{document}
\maketitle

\section*{Ex 3:}
\subsection*{a.}
$$ 3i = 3\cdot e^{\left(\frac{\pi}{2}+2k\pi\right)i} $$
$$\qquad = e^{ln(3)} \cdot e^{\left(\frac{\pi}{2}+2k\pi\right)i}$$
$$\qquad = e^{ln(3) + \left(\frac{\pi}{2} + 2k\pi \right)i}$$
\subsection*{b}
$$4+4i = 4\sqrt{2} \cdot e^{\left(\frac{\pi}{4}+2k\pi\right)i}$$
$$\qquad = e^{ln{4\sqrt{2}}} \cdot e^{\left(\frac{\pi}{4}+2k\pi\right)i}$$
$$\qquad = e^{ln{4\sqrt{2}} + \left(\frac{\pi}{4}+2k\pi\right)i}$$
\subsection*{c}
$$1+i\sqrt{3} = 2 \cdot e^{\left(\frac{\pi}{3}+2k\pi\right)i}$$
$$\qquad = e^{ln{2}} \cdot e^{\left(\frac{\pi}{3}+2k\pi\right)i}$$
$$\qquad = e^{ln{2} + \left(\frac{\pi}{3}+2k\pi\right)i}$$
\subsection*{d}

\section*{5}
$$p(z) = z^4 - 4z^3 + 14z^2 - 4z + 13$$
$$= z^4 +14z^2 + 13 -4z(z^2+1) $$
$$= (z^2+1)(z^2+13) - 4z(z^2+1) $$
$$= (z^2+1)(z^2-4z+13)$$
We get our zeros either from $z^2+1 = 0$ or $z^2-4z+13=0$
\begin{align*}
z^2+1  =  0 \\
z^2  =  -1 \\ 
z_{1/2}  =  \pm i
\end{align*}
and
\begin{align*}
    z^2-4z+13=0 \\
    (z-2)^2 - 4 + 13 = 0 \\
    (z-2)^2 = -9 \\ 
    z-2 = \pm 3i \\ 
    z = 2 \pm i3
\end{align*}

\begin{equation} \label{eq1}
\begin{split}
A & = \frac{\pi r^2}{2} \\
 & = \frac{1}{2} \pi r^2
\end{split}
\end{equation}

\end{document}